src/program_proof/memkv/urpc_spec.v
@@ -7,17 +7,17 @@ From Perennial.program_proof.memkv Require Import urpc_proof.
 
 Section rpc_global_defs.
 
-Context `{!rpcregG Σ}.
+Context `{!urpcregG Σ}.
 Context `{HPRE: !gooseGlobalGS Σ}.
 
 (* Higher-level interface for defining a handler with a given spec. *)
-Record RPCSpec :=
+Record uRPCSpec :=
   { spec_rpcid : u64;
     spec_ty : Type;
     spec_Pre : spec_ty → list u8 → iProp Σ;
     spec_Post : spec_ty → list u8 → list u8 → iProp Σ }.
 
-Program Definition RPCSpec_Spec (spec : RPCSpec) : savedSpecO Σ (list u8) (list u8) :=
+Program Definition uRPCSpec_Spec (spec : uRPCSpec) : savedSpecO Σ (list u8) (list u8) :=
   λ args, λne (Φ : list u8 -d> iPropO Σ), (∃ x : spec.(spec_ty),
     spec.(spec_Pre) x args ∗ (∀ rep, spec.(spec_Post) x args rep -∗ Φ rep))%I.
 Next Obligation. (* FIXME solve_propert solved a very similar goal, why not this? *)
@@ -25,57 +25,57 @@ Next Obligation. (* FIXME solve_propert solved a very similar goal, why not this
   intros x. f_equiv. f_equiv. intros rep. f_equiv. apply HΦ.
 Qed.
 
-Definition handler_rpc_spec Γsrv (host:u64) (spec : RPCSpec) :=
-  handler_spec Γsrv host spec.(spec_rpcid) (RPCSpec_Spec spec).
+Definition handler_urpc_spec Γsrv (host:u64) (spec : uRPCSpec) :=
+  handler_spec Γsrv host spec.(spec_rpcid) (uRPCSpec_Spec spec).
 
 (* We define a custom type for a list of RPC specs in order to state lemmas
    about initializing a collection of handler_is facts. Unfortunately, using the
    standard list type leads to a universe error if the spec_ty field contains an
    iProp Σ, which turns out to be rather common. *)
 
-Inductive RPCSpecList : Type :=
-| spec_nil : RPCSpecList
-| spec_cons (x: RPCSpec) (l: RPCSpecList) : RPCSpecList.
+Inductive uRPCSpecList : Type :=
+| spec_nil : uRPCSpecList
+| spec_cons (x: uRPCSpec) (l: uRPCSpecList) : uRPCSpecList.
 
-Fixpoint dom_RPCSpecList (l:  RPCSpecList) : gset u64 :=
+Fixpoint dom_uRPCSpecList (l:  uRPCSpecList) : gset u64 :=
   match l with
   | spec_nil => ∅
-  | spec_cons x l => {[ spec_rpcid x ]} ∪ dom_RPCSpecList l
+  | spec_cons x l => {[ spec_rpcid x ]} ∪ dom_uRPCSpecList l
   end.
 
-Fixpoint handler_RPCSpecList γ host (l : RPCSpecList) :=
+Fixpoint handler_uRPCSpecList γ host (l : uRPCSpecList) :=
   match l with
   | spec_nil => True%I
   | spec_cons x l =>
-    (handler_rpc_spec γ host x ∗
-                handler_RPCSpecList γ host l)%I
+    (handler_urpc_spec γ host x ∗
+                handler_uRPCSpecList γ host l)%I
   end.
 
-Fixpoint RPCSpecList_wf (l : RPCSpecList) : Prop :=
+Fixpoint uRPCSpecList_wf (l : uRPCSpecList) : Prop :=
   match l with
   | spec_nil => True
   | spec_cons x l =>
-    (spec_rpcid x ∉ dom_RPCSpecList l) ∧ RPCSpecList_wf l
+    (spec_rpcid x ∉ dom_uRPCSpecList l) ∧ uRPCSpecList_wf l
   end.
 
-Lemma handler_is_init_list (host : chan) (specs: RPCSpecList) (Hwf: RPCSpecList_wf specs) :
+Lemma handler_is_init_list (host : chan) (specs: uRPCSpecList) (Hwf: uRPCSpecList_wf specs) :
    host c↦ ∅ ={⊤}=∗ ∃ γ,
-   handlers_dom γ (dom_RPCSpecList specs) ∗
-   handler_RPCSpecList γ host specs.
+   handlers_dom γ (dom_uRPCSpecList specs) ∗
+   handler_uRPCSpecList γ host specs.
 Proof.
   iIntros "Hchan".
   iMod (map_init (∅ : gmap u64 gname)) as (γmap) "Hmap_ctx".
-  iMod (own_alloc (to_agree (dom_RPCSpecList specs : leibnizO (gset u64)))) as (γdom) "#Hdom".
+  iMod (own_alloc (to_agree (dom_uRPCSpecList specs : leibnizO (gset u64)))) as (γdom) "#Hdom".
   { econstructor. }
   set (Γsrv := {| scmap_name := γmap; scset_name := γdom |}).
   iMod (inv_alloc urpc_serverN _ ((server_chan_inner host Γsrv)) with "[Hchan]") as "#Hinv".
   { iNext. iExists _. iFrame.
     rewrite big_sepS_empty //. }
   iExists Γsrv.
-  iAssert (∀ specs', ⌜ RPCSpecList_wf specs' ⌝ ∗ ⌜ dom_RPCSpecList specs' ⊆  dom_RPCSpecList specs ⌝ →
-           |==> ∃ gnames : gmap u64 gname, ⌜ dom (gset _) gnames = dom_RPCSpecList specs' ⌝ ∗
+  iAssert (∀ specs', ⌜ uRPCSpecList_wf specs' ⌝ ∗ ⌜ dom_uRPCSpecList specs' ⊆  dom_uRPCSpecList specs ⌝ →
+           |==> ∃ gnames : gmap u64 gname, ⌜ dom (gset _) gnames = dom_uRPCSpecList specs' ⌝ ∗
            map_ctx (scmap_name Γsrv) 1 gnames ∗
-           handler_RPCSpecList Γsrv host specs')%I with "[Hmap_ctx]" as "H"; last first.
+           handler_uRPCSpecList Γsrv host specs')%I with "[Hmap_ctx]" as "H"; last first.
   { iMod ("H" with "[]") as (?) "(_&_&$)"; eauto. }
   iIntros (specs').
   iInduction specs' as [| hd spec] "IH".
@@ -86,7 +86,7 @@ Proof.
     { iPureIntro. split.
       - destruct Hwf' as (_&?); eauto.
       - etransitivity; last eassumption. set_solver. }
-    iMod (saved_spec_alloc (RPCSpec_Spec hd)) as (γsave) "#Hsaved".
+    iMod (saved_spec_alloc (uRPCSpec_Spec hd)) as (γsave) "#Hsaved".
     iMod (map_alloc_ro (spec_rpcid hd) γsave
             with "Hmap_ctx") as "(Hmap_ctx&#Hsaved_name)"; auto.
     { apply not_elem_of_dom. destruct (Hwf') as (?&?). rewrite Hdom. eauto. }
