src/program_proof/memkv/memkv_shard_start_proof.v
@@ -5,7 +5,7 @@ From Perennial.program_proof.memkv Require Export memkv_shard_definitions memkv_
 
 Section memkv_shard_start_proof.
 
-Context `{!heapGS Σ, rpcG Σ ShardReplyC, rpcregG Σ, kvMapG Σ}.
+Context `{!heapGS Σ, rpcG Σ ShardReplyC, urpcregG Σ, kvMapG Σ}.
 
 Lemma wp_KVShardServer__Start (s:loc) (host : u64) γ :
 handlers_dom γ.(urpc_gn) {[ U64 0; U64 1; U64 2; U64 3; U64 4; U64 5 ]} -∗
